More correct indistinguishability + better stack representation
Fixed at least 2 bugs in indistinguishability,
one is for stacks and Leo knew about it already
the second one is in how stack frames are compared
(registers used to be ignored!)

Probably managed to break other things since testing now fails.
Will debug soon, I hope, but any help welcome.

ifc/extended/Machine/Machine.v
@@ -112,11 +112,15 @@ Definition register := Atom.
 Definition regSet := list register.
 
 (* Stack *)
-Inductive Stack :=
-  | Mty                                       (* empty stack *)
-  | RetCons (pc_l:Ptr_atom * Label * regSet * regId) (s:Stack).
-   (* stack frame marker cons (with return pc and protecting label) *)
-Infix ":::" := RetCons (at level 60, right associativity).
+Record StackFrame := SF {
+  sf_return_addr : Ptr_atom;
+  sf_saved_regs : regSet;
+  sf_result_reg : regId;
+  sf_result_lab : Label
+}.
+
+Inductive Stack : Type := ST : list StackFrame -> Stack.
+Definition unStack s := let 'ST xs := s in xs.
 
 Class Join (t :Type) := {
   join_label: t -> Label -> t
@@ -465,7 +469,7 @@ Inductive step (t : table) : State -> State -> Prop :=
      (TMU : run_tmr t OpBCall <|La; K|> Lpc = Some (Some rl, rpcl)),
      step t
        (St im μ σ r pc)
-       (St im μ (((PAtm (j+1) rl), B, r, r3) ::: σ) r (PAtm addr rpcl))
+       (St im μ (ST (SF (PAtm (j+1) rl) r r3 B :: (unStack σ))) r (PAtm addr rpcl))
  | step_bret: forall im μ σ pc a r r' r'' r1 R pc' B j j' LPC LPC' rl rpcl
      (PC: pc  = PAtm j  LPC)
      (PC': pc' = PAtm j' LPC')
@@ -474,7 +478,7 @@ Inductive step (t : table) : State -> State -> Prop :=
      (TMU : run_tmr t OpBRet <|R; B; LPC'|> LPC = Some (Some rl, rpcl))
      (RES : registerUpdate r' r1 (a @ rl) = Some r''),
      step t
-       (St im μ ((pc',B,r',r1) ::: σ) r pc)
+       (St im μ (ST (SF pc' r' r1 B :: (unStack σ))) r pc)
        (St im μ σ r'' (PAtm j' rpcl))
  | step_alloc: forall im μ μ' σ pc r r' r1 r2 r3 i K Ll K' rl rpcl j LPC dfp
      (PC: pc = PAtm j LPC)
@@ -667,21 +671,21 @@ Definition fstep t (st:State) : option State :=
         | Some (Vint addr @ Ll), Some (Vlab B @ K) =>
           match run_tmr t OpBCall <|Ll; K|> LPC with
             | Some (Some rl, rpcl) =>
-              Some (St im μ (((PAtm (j+1) rl), B, r, r3) ::: σ) r
+              Some (St im μ (ST (SF (PAtm (j+1) rl) r r3 B :: (unStack σ))) r
                        (PAtm addr rpcl))
             | _ => None
           end
         | _, _ => None
       end
     | BRet =>
-      match σ with
-        | (PAtm jp' LPC', B, savedRegs, r1) ::: σ' =>
+      match unStack σ with
+        | SF (PAtm jp' LPC') savedRegs r1 B :: σ' =>
           do r1Cont <- registerContent r r1;
           let '(a @ R) := r1Cont in
           match run_tmr t OpBRet <|R; B; LPC'|> LPC with
             | Some (Some rl, rpcl) =>
               do r' <- registerUpdate savedRegs r1 (a @ rl);
-              Some (St im μ σ' r' (PAtm jp' rpcl))
+              Some (St im μ (ST σ') r' (PAtm jp' rpcl))
             | _ => None
           end
         | _ => None
